Move all uses of memory implementation to Memory
Now, Memory.v contains all theorems about the CompCert memory
model, so that no implementation details leak into the other
proofs of the compiler.

backend/Deadcodeproof.v
@@ -29,146 +29,20 @@ Qed.
 
 (** * Relating the memory states *)
 
-(** The [magree] predicate is a variant of [Mem.extends] where we
-  allow the contents of the two memory states to differ arbitrarily
-  on some locations.  The predicate [P] is true on the locations whose
-  contents must be in the [lessdef] relation. *)
+Local Notation locset := Mem.locset.
+Local Notation magree := Mem.magree.
 
-Definition locset := block -> Z -> Prop.
-
-Record magree (m1 m2: mem) (P: locset) : Prop := mk_magree {
-  ma_perm:
-    forall b ofs k p,
-    Mem.perm m1 b ofs k p ->
-    Mem.perm m2 b ofs k p;
-  ma_memval:
-    forall b ofs,
-    Mem.perm m1 b ofs Cur Readable ->
-    P b ofs ->
-    memval_lessdef (ZMap.get ofs (PMap.get b (Mem.mem_contents m1)))
-                   (ZMap.get ofs (PMap.get b (Mem.mem_contents m2)));
-  ma_nextblock:
-    Mem.nextblock m2 = Mem.nextblock m1
-}.
-
-Lemma magree_monotone:
-  forall m1 m2 (P Q: locset),
-  magree m1 m2 P ->
-  (forall b ofs, Q b ofs -> P b ofs) ->
-  magree m1 m2 Q.
-Proof.
-  intros. destruct H. constructor; auto.
-Qed.
-
-Lemma mextends_agree:
-  forall m1 m2 P, Mem.extends m1 m2 -> magree m1 m2 P.
-Proof.
-  intros. destruct H. destruct mext_inj. constructor; intros.
-- replace ofs with (ofs + 0) by omega. eapply mi_perm; eauto. auto.
-- exploit mi_memval; eauto. unfold inject_id; eauto.
-  rewrite Zplus_0_r. auto.
-- auto.
-Qed.
-
-Lemma magree_extends:
-  forall m1 m2 (P: locset),
-  (forall b ofs, P b ofs) ->
-  magree m1 m2 P -> Mem.extends m1 m2.
-Proof.
-  intros. destruct H0. constructor; auto. constructor; unfold inject_id; intros.
-- inv H0. rewrite Zplus_0_r. eauto.
-- inv H0. apply Zdivide_0.
-- inv H0. rewrite Zplus_0_r. eapply ma_memval0; eauto.
-Qed.
-
-Lemma magree_loadbytes:
-  forall m1 m2 P b ofs n bytes,
-  magree m1 m2 P ->
-  Mem.loadbytes m1 b ofs n = Some bytes ->
-  (forall i, ofs <= i < ofs + n -> P b i) ->
-  exists bytes', Mem.loadbytes m2 b ofs n = Some bytes' /\ list_forall2 memval_lessdef bytes bytes'.
-Proof.
-  assert (GETN: forall c1 c2 n ofs,
-    (forall i, ofs <= i < ofs + Z.of_nat n -> memval_lessdef (ZMap.get i c1) (ZMap.get i c2)) ->
-    list_forall2 memval_lessdef (Mem.getN n ofs c1) (Mem.getN n ofs c2)).
-  {
-    induction n; intros; simpl.
-    constructor.
-    rewrite inj_S in H. constructor.
-    apply H. omega.
-    apply IHn. intros; apply H; omega.
-  }
-Local Transparent Mem.loadbytes.
-  unfold Mem.loadbytes; intros. destruct H.
-  destruct (Mem.range_perm_dec m1 b ofs (ofs + n) Cur Readable); inv H0.
-  rewrite pred_dec_true. econstructor; split; eauto.
-  apply GETN. intros. rewrite nat_of_Z_max in H.
-  assert (ofs <= i < ofs + n) by xomega.
-  apply ma_memval0; auto.
-  red; intros; eauto.
-Qed.
-
-Lemma magree_load:
-  forall m1 m2 P chunk b ofs v,
-  magree m1 m2 P ->
-  Mem.load chunk m1 b ofs = Some v ->
-  (forall i, ofs <= i < ofs + size_chunk chunk -> P b i) ->
-  exists v', Mem.load chunk m2 b ofs = Some v' /\ Val.lessdef v v'.
-Proof.
-  intros. exploit Mem.load_valid_access; eauto. intros [A B].
-  exploit Mem.load_loadbytes; eauto. intros [bytes [C D]].
-  exploit magree_loadbytes; eauto. intros [bytes' [E F]].
-  exists (decode_val chunk bytes'); split.
-  apply Mem.loadbytes_load; auto.
-  apply val_inject_id. subst v. apply decode_val_inject; auto.
-Qed.
-
-Lemma magree_storebytes_parallel:
-  forall m1 m2 (P Q: locset) b ofs bytes1 m1' bytes2,
-  magree m1 m2 P ->
-  Mem.storebytes m1 b ofs bytes1 = Some m1' ->
-  (forall b' i, Q b' i ->
-                b' <> b \/ i < ofs \/ ofs + Z_of_nat (length bytes1) <= i ->
-                P b' i) ->
-  list_forall2 memval_lessdef bytes1 bytes2 ->
-  exists m2', Mem.storebytes m2 b ofs bytes2 = Some m2' /\ magree m1' m2' Q.
-Proof.
-  assert (SETN: forall (access: Z -> Prop) bytes1 bytes2,
-    list_forall2 memval_lessdef bytes1 bytes2 ->
-    forall p c1 c2,
-    (forall i, access i -> i < p \/ p + Z.of_nat (length bytes1) <= i -> memval_lessdef (ZMap.get i c1) (ZMap.get i c2)) ->
-    forall q, access q ->
-    memval_lessdef (ZMap.get q (Mem.setN bytes1 p c1))
-                   (ZMap.get q (Mem.setN bytes2 p c2))).
-  {
-    induction 1; intros; simpl.
-  - apply H; auto. simpl. omega.
-  - simpl length in H1; rewrite inj_S in H1.
-    apply IHlist_forall2; auto.
-    intros. rewrite ! ZMap.gsspec. destruct (ZIndexed.eq i p). auto.
-    apply H1; auto. unfold ZIndexed.t in *; omega.
-  }
-  intros.
-  destruct (Mem.range_perm_storebytes m2 b ofs bytes2) as [m2' ST2].
-  { erewrite <- list_forall2_length by eauto. red; intros.
-    eapply ma_perm; eauto.
-    eapply Mem.storebytes_range_perm; eauto. }
-  exists m2'; split; auto.
-  constructor; intros.
-- eapply Mem.perm_storebytes_1; eauto. eapply ma_perm; eauto.
-  eapply Mem.perm_storebytes_2; eauto.
-- rewrite (Mem.storebytes_mem_contents _ _ _ _ _ H0).
-  rewrite (Mem.storebytes_mem_contents _ _ _ _ _ ST2).
-  rewrite ! PMap.gsspec. destruct (peq b0 b).
-+ subst b0. apply SETN with (access := fun ofs => Mem.perm m1' b ofs Cur Readable /\ Q b ofs); auto.
-  intros. destruct H5. eapply ma_memval; eauto.
-  eapply Mem.perm_storebytes_2; eauto.
-  apply H1; auto.
-+ eapply ma_memval; eauto. eapply Mem.perm_storebytes_2; eauto. apply H1; auto.
-- rewrite (Mem.nextblock_storebytes _ _ _ _ _ H0).
-  rewrite (Mem.nextblock_storebytes _ _ _ _ _ ST2).
-  eapply ma_nextblock; eauto.
-Qed.
+Local Notation magree_storebytes_parallel := Mem.magree_storebytes_parallel.
+Local Notation magree_monotone := Mem.magree_monotone.
+Local Notation magree_load := Mem.magree_load.
+Local Notation magree_valid_access := Mem.magree_valid_access.
+Local Notation ma_perm := Mem.ma_perm.
+Local Notation magree_store_left := Mem.magree_store_left.
+Local Notation magree_extends := Mem.magree_extends.
+Local Notation magree_free := Mem.magree_free.
+Local Notation magree_loadbytes := Mem.magree_loadbytes.
+Local Notation magree_storebytes_left := Mem.magree_storebytes_left.
+Local Notation mextends_agree := Mem.mextends_agree.
 
 Lemma magree_store_parallel:
   forall m1 m2 (P Q: locset) chunk b ofs v1 m1' v2,
@@ -190,78 +64,6 @@ Proof.
   intros [m2' [SB2 AG]].
   exists m2'; split; auto.
   apply Mem.storebytes_store; auto.
-Qed.
-
-Lemma magree_storebytes_left:
-  forall m1 m2 P b ofs bytes1 m1',
-  magree m1 m2 P ->
-  Mem.storebytes m1 b ofs bytes1 = Some m1' ->
-  (forall i, ofs <= i < ofs + Z_of_nat (length bytes1) -> ~(P b i)) ->
-  magree m1' m2 P.
-Proof.
-  intros. constructor; intros.
-- eapply ma_perm; eauto. eapply Mem.perm_storebytes_2; eauto.
-- rewrite (Mem.storebytes_mem_contents _ _ _ _ _ H0).
-  rewrite PMap.gsspec. destruct (peq b0 b).
-+ subst b0. rewrite Mem.setN_outside. eapply ma_memval; eauto. eapply Mem.perm_storebytes_2; eauto.
-  destruct (zlt ofs0 ofs); auto. destruct (zle (ofs + Z.of_nat (length bytes1)) ofs0); try omega.
-  elim (H1 ofs0). omega. auto.
-+ eapply ma_memval; eauto. eapply Mem.perm_storebytes_2; eauto.
-- rewrite (Mem.nextblock_storebytes _ _ _ _ _ H0).
-  eapply ma_nextblock; eauto.
-Qed.
-
-Lemma magree_store_left:
-  forall m1 m2 P chunk b ofs v1 m1',
-  magree m1 m2 P ->
-  Mem.store chunk m1 b ofs v1 = Some m1' ->
-  (forall i, ofs <= i < ofs + size_chunk chunk -> ~(P b i)) ->
-  magree m1' m2 P.
-Proof.
-  intros. eapply magree_storebytes_left; eauto.
-  eapply Mem.store_storebytes; eauto.
-  intros. rewrite encode_val_length in H2.
-  rewrite <- size_chunk_conv in H2. apply H1; auto.
-Qed.
-
-Lemma magree_free:
-  forall m1 m2 (P Q: locset) b lo hi m1',
-  magree m1 m2 P ->
-  Mem.free m1 b lo hi = Some m1' ->
-  (forall b' i, Q b' i ->
-                b' <> b \/ ~(lo <= i < hi) ->
-                P b' i) ->
-  exists m2', Mem.free m2 b lo hi = Some m2' /\ magree m1' m2' Q.
-Proof.
-  intros.
-  destruct (Mem.range_perm_free m2 b lo hi) as [m2' FREE].
-  red; intros. eapply ma_perm; eauto. eapply Mem.free_range_perm; eauto.
-  exists m2'; split; auto.
-  constructor; intros.
-- (* permissions *)
-  assert (Mem.perm m2 b0 ofs k p). { eapply ma_perm; eauto. eapply Mem.perm_free_3; eauto. }
-  exploit Mem.perm_free_inv; eauto. intros [[A B] | A]; auto.
-  subst b0. eelim Mem.perm_free_2. eexact H0. eauto. eauto.
-- (* contents *)
-  rewrite (Mem.free_result _ _ _ _ _ H0).
-  rewrite (Mem.free_result _ _ _ _ _ FREE).
-  simpl. eapply ma_memval; eauto. eapply Mem.perm_free_3; eauto.
-  apply H1; auto. destruct (eq_block b0 b); auto.
-  subst b0. right. red; intros. eelim Mem.perm_free_2. eexact H0. eauto. eauto.
-- (* nextblock *)
-  rewrite (Mem.free_result _ _ _ _ _ H0).
-  rewrite (Mem.free_result _ _ _ _ _ FREE).
-  simpl. eapply ma_nextblock; eauto.
-Qed.
-
-Lemma magree_valid_access:
-  forall m1 m2 (P: locset) chunk b ofs p,
-  magree m1 m2 P ->
-  Mem.valid_access m1 chunk b ofs p ->
-  Mem.valid_access m2 chunk b ofs p.
-Proof.
-  intros. destruct H0; split; auto.
-  red; intros. eapply ma_perm; eauto.
 Qed.
 
 (** * Properties of the need environment *)
@@ -1015,7 +817,7 @@ Ltac UseTransfer :=
   exploit transfer_builtin_args_sound; eauto. intros (tvl & A & B & C & D).
   exploit external_call_mem_extends; eauto 2 with na.
   eapply magree_extends; eauto. intros. apply nlive_all.
-  intros (v' & tm' & P & Q & R & S & T).
+  intros (v' & tm' & P & Q & R & ST).
   econstructor; split.
   eapply exec_Ibuiltin; eauto.
   apply eval_builtin_args_preserved with (ge1 := ge); eauto. exact symbols_preserved.
@@ -1066,7 +868,7 @@ Ltac UseTransfer :=
 
 - (* external function *)
   exploit external_call_mem_extends; eauto.
-  intros (res' & tm' & A & B & C & D & E).
+  intros (res' & tm' & A & B & C & DE).
   simpl in FUN. inv FUN.
   econstructor; split.
   econstructor; eauto.
