backend/Stackingproof.v
@@ -1837,7 +1837,7 @@ Proof.
   by omega.
   destruct EITHER.
   replace ofs with ((ofs - fe_stack_data fe) + fe_stack_data fe) by omega.
-  eapply Mem.perm_inject with (f := j). eapply agree_inj; eauto. eauto.
+  eapply Mem.perm_inject. 2: eassumption. eapply agree_inj; eauto. eauto.
   eapply Mem.free_range_perm; eauto. omega.
   eapply agree_perm; eauto.
   (* inject after free *)
